src/arch/x64/X64.Print_s.fst
@@ -153,14 +153,15 @@ let print_ins (ins:ins) (p:printer) =
   | And64 dst src -> p.ins_name "  and" [dst; src] ^ print_ops dst src
   | Shr64 dst amt -> p.ins_name "  shr" [dst; amt] ^ print_shift dst amt
   | Shl64 dst amt -> p.ins_name "  shl" [dst; amt] ^ print_shift dst amt
-  | Paddd dst src           -> " paddd "      ^ print_xmms dst src
+  | Paddd dst src          -> "  paddd "      ^ print_xmms dst src
   | Pxor dst src           -> "  pxor "       ^ print_xmms dst src
   | Pslld dst amt          -> "  pslld "      ^ print_pair (print_xmm dst) (string_of_int amt)
   | Psrld dst amt          -> "  psrld "      ^ print_pair (print_xmm dst) (string_of_int amt)
+  | Pshufb dst src         -> "  pshufb "     ^ print_xmms dst src
   | Pshufd dst src count   -> "  pshufd "     ^ print_pair (print_xmms dst src) (print_imm8 count)
   | Pinsrd dst src index   -> "  pinsrd "     ^ print_pair (print_xmm_op dst src) (print_imm8 index)
-  | VPSLLDQ dst src count  -> "   vpslldq "   ^ print_pair (print_xmms dst src) (print_imm8 count)
-  | MOVDQU dst src         -> "   movdqu "    ^ print_pair (print_mov128_op dst p) (print_mov128_op src p)
+  | VPSLLDQ dst src count  -> "  vpslldq "    ^ print_pair (print_xmms dst src) (print_imm8 count)
+  | MOVDQU dst src         -> "  movdqu "     ^ print_pair (print_mov128_op dst p) (print_mov128_op src p)
   | Pclmulqdq dst src imm  -> "  pclmulqdq "  ^ print_pair (print_xmms dst src) (string_of_int imm)
   | AESNI_enc dst src      -> "  aesenc "     ^ print_xmms dst src
   | AESNI_enc_last dst src -> "  aesenclast " ^ print_xmms dst src
